\documentclass[a4paper,10pt]{article}

\usepackage{amsmath}
\usepackage{amssymb}
\usepackage{amsthm}
\usepackage{xfrac}
\usepackage[all]{xy}
\usepackage{mathtools}
\usepackage{graphicx}
\usepackage{fullpage}
\usepackage{hyperref}
\usepackage[utf8x]{inputenc}
\usepackage[italian]{babel}

\usepackage{ulem}

\setlength{\parindent}{0in}

\newcounter{counter1}

\theoremstyle{plain}
\newtheorem{myteo}[counter1]{Teorema}
\newtheorem{mylem}[counter1]{Lemma}
\newtheorem{mypro}[counter1]{Proposizione}
\newtheorem{mycor}[counter1]{Corollario}
\newtheorem*{myteo*}{Teorema}
\newtheorem*{mylem*}{Lemma}
\newtheorem*{mypro*}{Proposizione}
\newtheorem*{mycor*}{Corollario}

\theoremstyle{definition}
\newtheorem{mydef}[counter1]{Definizione}
\newtheorem{myes}[counter1]{Esempio}
\newtheorem{myex}[counter1]{Esercizio}
\newtheorem*{mydef*}{Definizione}
\newtheorem*{myes*}{Esempio}
\newtheorem*{myex*}{Esercizio}

\theoremstyle{remark}
\newtheorem{mynot}[counter1]{Nota}
\newtheorem{myoss}[counter1]{Osservazione}
\newtheorem*{mynot*}{Nota}
\newtheorem*{myoss*}{Osservazione}

\newcommand{\obar}[1]{\overline{#1}}
\newcommand{\ubar}[1]{\underline{#1}}

\newcommand{\set}[1]{\left\{#1\right\}}
\newcommand{\pa}[1]{\left(#1\right)}
\newcommand{\ang}[1]{\left<#1\right>}
\newcommand{\bra}[1]{\left[#1\right]}
\newcommand{\abs}[1]{\left|#1\right|}
\newcommand{\norm}[1]{\left\|#1\right\|}

\newcommand{\pfrac}[2]{\pa{\frac{#1}{#2}}}
\newcommand{\bfrac}[2]{\bra{\frac{#1}{#2}}}
\newcommand{\psfrac}[2]{\pa{\sfrac{#1}{#2}}}
\newcommand{\bsfrac}[2]{\bra{\sfrac{#1}{#2}}}

\newcommand{\der}[2]{\frac{\partial #1}{\partial #2}}
\newcommand{\pder}[2]{\pfrac{\partial #1}{\partial #2}}
\newcommand{\sder}[2]{\sfrac{\partial #1}{\partial #2}}
\newcommand{\psder}[2]{\psfrac{\partial #1}{\partial #2}}

\newcommand{\intl}{\int \limits}

\DeclareMathOperator{\de}{d}
\DeclareMathOperator{\id}{Id}
\DeclareMathOperator{\len}{len}


\title{Conti per la L-curve}
\author{Enrico Polesel}
\date{\today}

\begin{document}
\maketitle

\section{Formule note}

\begin{equation}
  \Delta v = \sum _{m=1} ^M \sigma _m g_\alpha \pa{\sigma_m ^2 }
  \ang{T,w_m} u_m
\end{equation}

\begin{equation}
  g_\alpha \pa{\sigma_m ^2 } = \pa{ \sigma _m ^2 + \alpha \beta _m ^2
  } ^ {-1}
\end{equation}

\begin{equation}
  \kappa (\alpha) = \frac{ \rho ' \eta ''  - \rho '' \eta '}{
    \pa{\pa{\rho ' } ^2 + \pa{ \eta ' } ^2 } ^ {\sfrac{3}{2}}}
\end{equation}

\begin{equation}
  \obar{\eta} ^2 (\alpha) = \norm{ \alpha D \Delta v } _2 ^2
\end{equation}

\begin{equation}
  \obar{\rho} ^2 (\alpha) = \norm{ A \Delta v - T}_2 ^2
\end{equation}

\begin{align*}
  \eta = \log \obar{\eta} \\
  \rho = \log \obar{\rho} \\
  A = W \Sigma U ^T \\
  D^T D \Delta v = \sum _{m=1} ^ M \beta _m ^2 \ang{ \delta v , u_m }
  u_m \\
  D = WBU^T
\end{align*}


\section{$\rho$ e $\eta$}

\subsection{$\rho$}

\begin{align*}
  \obar{\rho} ^2 (\alpha) =& \norm{ A \Delta v - T}_2 ^2 = \\
  =& \norm{ W \Sigma U ^T \Delta v - T}_2 ^2 = \\
  =& \norm{ \Sigma U ^T \Delta v - W^T T}_2 ^2 = \\
  = & \norm{ \Sigma U ^T \Delta v - \sum_{m=1} ^M \ang{w_m, T}e_m }_2
  ^2 = \\
  = & \norm{ \sum _{m=1} ^M \pa{ \sigma _m \ang{u_m, \Delta v} e_m -
      \ang{w_m, T}e_m } }_2 ^2 = \\
  = & \sum _{m=1} ^M \pa{ \sigma _m \ang{u_m, \Delta v} -
    \ang{w_m, T} } ^2 = \\
  = & \sum _{m=1} ^M \pa{ \sigma _m \ang{u_m , \sum _{n=1} ^M \sigma
      _n g_\alpha \pa{\sigma_n ^2 } \ang{T,w_n} u_n} - \ang{w_m, T} }
  ^2 = \\
  = & \sum _{m=1} ^M \pa{ \sigma _m ^2 g_\alpha \pa{\sigma_m ^2
    } \ang{T,w_m} - \ang{w_m, T} }^2 = \\
  = &\sum _{m=1} ^M \bra{ \ang{w_m, T} \pa{ \sigma _m ^2 g_\alpha
      \pa{\sigma_m ^2 } -1 }  } ^2 = \\
  = & \sum _{m=1} ^M \bra{ \ang{w_m, T} \pa{ \sigma _m ^2 \pa{ \sigma
        _m ^2 + \alpha \beta _m ^2 } ^ {-1}  - 1 } } ^2 = \\
  = & \sum _{m=1} ^M \bra{ \ang{w_m, T} \pa{ \frac{\sigma _m ^2}{
        \sigma _m ^2 + \alpha \beta _m ^2 } - 1 } } ^2
\end{align*}

\begin{align*}
  \rho (\alpha) = & \log \sqrt { \sum _{m=1} ^M \bra{ \ang{w_m, T} \pa{
        \frac{\sigma _m ^2}{ \sigma
          _m ^2 + \alpha \beta _m ^2 } - 1 } } ^2  } = \\
  = & \frac{1}{2} \log { \sum _{m=1} ^M \bra{ \ang{w_m, T} \pa{
        \frac{\sigma _m ^2}{ \sigma _m ^2 + \alpha \beta _m ^2 } - 1 }
    } ^2 }
\end{align*}

\begin{align*}
  \rho ' (\alpha) = & \frac{1}{2} \frac{\sum _{m=1} ^M 2
    \bra{\ang{w_m, T} \pa{ \frac{\sigma _m ^2}{ \sigma _m ^2 + \alpha
          \beta _m ^2 } - 1}\bra{- \ang{w_m, T} \sigma _m ^2
        \frac{\beta _m ^2}{\pa{\sigma _m ^2 + \alpha \beta_m ^2}^2} }
    }} { \sum _{m=1} ^M \bra{ \ang{w_m, T} \pa{ \frac{\sigma _m ^2}{
          \sigma
          _m ^2 + \alpha \beta _m ^2 } - 1 }  } ^2  } = \\
  = & \frac{\sum _{m=1} ^M \ang{w_m, T}^2 \bra{ \frac{\alpha \beta _m
        ^2}{ \sigma _m ^2 + \alpha \beta _m ^2 } \frac{ \sigma _m ^2
        \beta _m ^2}{\pa{\sigma _m ^2 + \alpha \beta_m ^2}^2} }} {
    \sum _{m=1} ^M \bra{ \ang{w_m, T} \pa{ \frac{\sigma _m ^2}{ \sigma
          _m ^2 + \alpha \beta _m ^2 } - 1 }  } ^2  } = \\
  = & - \frac{\sum _{m=1} ^M \ang{w_m, T}^2 \bra{ \frac{\alpha \sigma _m
        ^2 \beta _m ^4}{\pa{\sigma _m ^2 + \alpha \beta_m ^2}^3} }} {
    \sum _{m=1} ^M \bra{ \ang{w_m, T}  \frac{\alpha \beta _m ^2}{ \sigma
          _m ^2 + \alpha \beta _m ^2 }   } ^2  } \\
\end{align*}

\begin{align*}
  \rho '' (\alpha) = & - \frac{ \bra{\sum _{m=1} ^M \pa{ \ang{w_m, T}
        \frac{\alpha \beta _m ^2}{ \sigma _m ^2 + \alpha \beta _m ^2 }
      } ^2} \bra{ \sum _{m=1} ^M \ang{w_m, T}^2 \frac{\sigma _m ^2
        \beta _m ^4 \pa{ \sigma _m ^2 + \alpha \beta _m ^2 } ^3 -3
        \pa{ \sigma _m ^2 + \alpha \beta _m ^2} ^2 \beta_m ^2 \alpha
        \sigma _m ^2 \beta _m ^4 }{\pa{ \sigma _m ^2 + \alpha \beta _m
          ^2 }^6} }}{\bra{\sum _{m=1} ^M \pa{
        \ang{w_m, T} \frac{\alpha \beta _m ^2}{ \sigma _m ^2 + \alpha
          \beta _m ^2 } } ^2} ^2} + \\
  & + \frac{\bra{2\sum _{m=1} ^M \ang{w_m, T}^2 \pa{
        \frac{\alpha \sigma _m ^2 \beta _m ^4}{\pa{\sigma _m ^2 +
            \alpha \beta_m ^2}^3} }}^2 } {\bra{\sum _{m=1} ^M \pa{
        \ang{w_m, T} \frac{\alpha \beta _m ^2}{ \sigma _m ^2 + \alpha
          \beta _m ^2 } } ^2} ^2 } = \\
  = & \frac{ \bra{2\sum _{m=1} ^M \ang{w_m, T}^2 \pa{
        \frac{\alpha \sigma _m ^2 \beta _m ^4}{\pa{\sigma _m ^2 +
            \alpha \beta_m ^2}^3} }}^2 - \bra{\sum _{m=1} ^M \pa{ \ang{w_m, T}
        \frac{\alpha \beta _m ^2}{ \sigma _m ^2 + \alpha \beta _m ^2 }
      } ^2} \bra{ \sum _{m=1} ^M \ang{w_m, T}^2 \frac{\sigma _m ^2
        \beta _m ^4 \pa{ \sigma _m ^2 -2 \alpha \beta _m ^2  }
        }{\pa{ \sigma _m ^2 + \alpha \beta _m
          ^2 }^4} }}{\bra{\sum _{m=1} ^M \pa{
        \ang{w_m, T} \frac{\alpha \beta _m ^2}{ \sigma _m ^2 + \alpha
          \beta _m ^2 } } ^2} ^2}
\end{align*}

\begin{align*}
  f(\alpha) = \sum _{m=1} ^M \bra{ \ang{w_m, T} \pa{ \frac{\sigma _m
        ^2}{ \sigma _m ^2 + \alpha \beta _m ^2 } - 1 } } ^2 =  \sum
  _{m=1} ^M \bra{ \ang{w_m, T} \frac{\alpha \beta _m ^2}{ \sigma _m ^2
        + \alpha \beta _m ^2 }  } ^2
\end{align*}

\begin{align*}
  f ' (\alpha) = - 2 \sum _{m=1} ^M \ang{w_m, T}^2 \bra{ \frac{\alpha
      \sigma _m ^2 \beta _m ^4}{\pa{\sigma _m ^2 + \alpha \beta_m
        ^2}^3} }
\end{align*}

\begin{align*}
  f '' (\alpha) = -2 \sum _{m=1} ^M \ang{w_m, T}^2 \frac{\sigma _m ^2
        \beta _m ^4 \pa{ \sigma _m ^2 -2 \alpha \beta _m ^2  }
        }{\pa{ \sigma _m ^2 + \alpha \beta _m
          ^2 }^4}
\end{align*}

\begin{align*}
  \rho '(\alpha) = \frac{1}{2} \frac{f'(\alpha)}{\sqrt{f(\alpha)}}
\end{align*}

\begin{align*}
  \rho ''(\alpha) = \frac{1}{4} \frac{2 f''(\alpha) f(\alpha) - \pa{
      f'(\alpha)} ^2 }{\pa{f(\alpha)} ^{\sfrac{3}{2}}}
\end{align*}

\subsection{$\eta$}

\begin{align*}
  \obar{\eta}^2(\alpha ) = & \norm{ \alpha D \Delta v } _2 ^2 =  \\
  = & \norm{ \alpha WBU^T \Delta v } _2 ^2 =\\
  = & \norm{ \alpha B U^T \Delta v } _2 ^2 =\\
  = & \norm{ \sum _{m=1} ^M \beta _m \ang{ u_m , \Delta v} e_m } _2 ^2
  = \\
  = & \sum _{m=1} ^M \bra{ \beta _m \ang{ u_m , \Delta v} } ^2 = \\
  = & \sum _{m=1} ^M \bra{ \beta _m \ang{ u_m , \sum _{n=1} ^M \sigma
      _n g_\alpha \pa{\sigma_n ^2 } \ang{T,w_n} u_n} } ^2 = \\
  = & \sum _{m=1} ^M \bra{ \beta _m \sigma
    _m g_\alpha \pa{\sigma_m ^2 } \ang{T,w_m}  } ^2 = \\
  = & \sum _{m=1} ^M \bra{ \frac{ \beta _m \sigma
    _m}{\sigma _m ^2 + \alpha \beta _m ^2}  \ang{T,w_m}  } ^2 \\
\end{align*}

\begin{align*}
  \eta = & \log \sqrt{ \sum _{m=1} ^M \bra{ \frac{ \beta _m \sigma
        _m}{\sigma _m ^2 + \alpha \beta _m ^2} \ang{T,w_m} } ^2 } =
  \\
  = & \frac{1}{2} \log \sum _{m=1} ^M \bra{ \frac{ \beta _m \sigma
      _m}{\sigma _m ^2 + \alpha \beta _m ^2} \ang{T,w_m} } ^2
\end{align*}

\begin{align*}
  \eta ' (\alpha) = & \frac{1}{2} \frac{2 \sum _{m=1} ^M \bra{\frac{
        \beta _m \sigma _m}{\sigma _m ^2 + \alpha \beta _m ^2}
      \ang{T,w_m}}\bra{- \ang{T,w_m} \beta _m \sigma _m \frac{\beta_m
        ^2}{\pa{ \sigma _m ^2 + \alpha \beta _m ^2} ^{2} }} }{ \sum
    _{m=1} ^M \bra{ \frac{ \beta _m \sigma _m}{\sigma _m ^2 +
        \alpha \beta _m ^2} \ang{T,w_m} } ^2} = \\
  = & - \frac{ \sum _{m=1} ^M \bra{\ang{T,w_m}^2 \frac{ \beta _m ^4
        \sigma _m ^2 }{\pa{\sigma _m ^2 + \alpha \beta _m ^2} ^3 } }}
  { \sum _{m=1} ^M \bra{ \frac{ \beta _m \sigma _m}{\sigma _m ^2 +
        \alpha \beta _m ^2} \ang{T,w_m} } ^2} \\
\end{align*}

\begin{align*}
  \eta '' (\alpha) = & - \frac{ \bra{ \sum _{m=1} ^M \pa{ \frac{ \beta
          _m \sigma _m}{\sigma _m ^2 + \alpha \beta _m ^2} \ang{T,w_m}
      } ^2} \bra{ -3 \sum _{m=1} ^M \ang{T,w_m}^2 \frac{\beta _m ^6
        \sigma _m ^2 }{ \pa { \sigma _m ^2 + \alpha \beta _m ^2 } ^4 }
    } - \bra{2\sum _{m=1} ^M \pa{\ang{T,w_m}^2 \frac{ \beta _m ^4
          \sigma _m ^2 }{\pa{\sigma _m ^2 + \alpha \beta _m ^2} ^3 }
      }}^2 } { \bra{ \sum _{m=1} ^M \pa{ \frac{ \beta _m \sigma
          _m}{\sigma _m ^2 + \alpha \beta _m ^2}
        \ang{T,w_m} } ^2}^2 } = \\
  =& \frac{ \bra{2\sum _{m=1} ^M \pa{\ang{T,w_m}^2 \frac{ \beta _m
          ^4 \sigma _m ^2 }{\pa{\sigma _m ^2 + \alpha \beta _m ^2} ^3
        } }}^2 +3 \bra{ \sum _{m=1} ^M \pa{ \frac{ \beta _m \sigma
          _m}{\sigma _m ^2 + \alpha \beta _m ^2} \ang{T,w_m} } ^2}
    \bra{ \sum _{m=1} ^M \ang{T,w_m}^2 \frac{\beta _m ^6 \sigma _m ^2
      }{ \pa { \sigma _m ^2 + \alpha \beta _m ^2 } ^4 } } } { \bra{
      \sum _{m=1} ^M \pa{ \frac{ \beta _m \sigma _m}{\sigma _m ^2 +
          \alpha \beta _m ^2} \ang{T,w_m} } ^2}^2 }
\end{align*}

\begin{align*}
  h(\alpha) = \sum _{m=1} ^M \bra{ \frac{ \beta _m \sigma _m}{\sigma
      _m ^2 + \alpha \beta _m ^2} \ang{T,w_m} } ^2
\end{align*}

\begin{align*}
  h'(\alpha) = - 2 \sum _{m=1} ^M \bra{\ang{T,w_m}^2 \frac{ \beta _m
      ^4 \sigma _m ^2 }{\pa{\sigma _m ^2 + \alpha \beta _m ^2} ^3 } }
\end{align*}

\begin{align*}
  h''(\alpha) = 6 \sum _{m=1} ^M \ang{T,w_m}^2 \frac{\beta _m ^6 \sigma _m ^2
      }{ \pa { \sigma _m ^2 + \alpha \beta _m ^2 } ^4 }
\end{align*}

\begin{align*}
  \eta '(\alpha) = \frac{1}{2} \frac{h'(\alpha)}{\sqrt{h(\alpha)}}
\end{align*}

\begin{align*}
  \eta ''(\alpha) = \frac{1}{4} \frac{2 h''(\alpha) h(\alpha) - \pa{
      h'(\alpha)} ^2 }{\pa{h(\alpha)} ^{\sfrac{3}{2}}}
\end{align*}

\section{$\kappa$}

% \begin{align*}
%   \kappa (\alpha) = \frac{ 
%  { - \frac{\sum _{m=1} ^M \ang{w_m, T}^2 \bra{ \frac{\alpha \sigma _m
%         ^2 \beta _m ^4}{\pa{\sigma _m ^2 + \alpha \beta_m ^2}^3} }} {
%     \sum _{m=1} ^M \bra{ \ang{w_m, T}  \frac{\alpha \beta _m ^2}{ \sigma
%           _m ^2 + \alpha \beta _m ^2 }   } ^2  } }
%  { \frac{ \bra{2\sum _{m=1} ^M \pa{\ang{T,w_m}^2 \frac{ \beta _m
%           ^4 \sigma _m ^2 }{\pa{\sigma _m ^2 + \alpha \beta _m ^2} ^3
%         } }}^2 - \bra{ \sum _{m=1} ^M \pa{ \frac{ \beta _m \sigma
%           _m}{\sigma _m ^2 + \alpha \beta _m ^2} \ang{T,w_m} } ^2}
%     \bra{ \sum _{m=1} ^M \ang{T,w_m}^2 \frac{\beta _m ^6 \sigma _m ^2
%       }{ \pa { \sigma _m ^2 + \alpha \beta _m ^2 } ^4 } } } { \bra{
%       \sum _{m=1} ^M \pa{ \frac{ \beta _m \sigma _m}{\sigma _m ^2 +
%           \alpha \beta _m ^2} \ang{T,w_m} } ^2}^2 } } }
% {    \pa{\pa{
%  { - \frac{\sum _{m=1} ^M \ang{w_m, T}^2 \bra{ \frac{\alpha \sigma _m
%         ^2 \beta _m ^4}{\pa{\sigma _m ^2 + \alpha \beta_m ^2}^3} }} {
%     \sum _{m=1} ^M \bra{ \ang{w_m, T}  \frac{\alpha \beta _m ^2}{ \sigma
%           _m ^2 + \alpha \beta _m ^2 }   } ^2  } }
% } ^2 + \pa{ 
%  { - \frac{ \sum _{m=1} ^M \bra{\ang{T,w_m}^2 \frac{ \beta _m ^4
%         \sigma _m ^2 }{\pa{\sigma _m ^2 + \alpha \beta _m ^2} ^3 } }}
%   { \sum _{m=1} ^M \bra{ \frac{ \beta _m \sigma _m}{\sigma _m ^2 +
%         \alpha \beta _m ^2} \ang{T,w_m} } ^2} }
%  } ^2 } ^ {\sfrac{3}{2}}
% } \\
% +
%   \frac{{ \frac{ \bra{2\sum _{m=1} ^M \ang{w_m, T}^2 \pa{
%         \frac{\alpha \sigma _m ^2 \beta _m ^4}{\pa{\sigma _m ^2 +
%             \alpha \beta_m ^2}^3} }}^2 - \bra{\sum _{m=1} ^M \pa{ \ang{w_m, T}
%         \frac{\alpha \beta _m ^2}{ \sigma _m ^2 + \alpha \beta _m ^2 }
%       } ^2} \bra{ \sum _{m=1} ^M \ang{w_m, T}^2 \frac{\sigma _m ^2
%         \beta _m ^4 \pa{ \sigma _m ^2 + \alpha \beta _m ^2  -3 \alpha }
%         }{\pa{ \sigma _m ^2 + \alpha \beta _m
%           ^2 }^4} }}{\bra{\sum _{m=1} ^M \pa{
%         \ang{w_m, T} \frac{\alpha \beta _m ^2}{ \sigma _m ^2 + \alpha
%           \beta _m ^2 } } ^2} ^2} }
%   {  \frac{ \sum _{m=1} ^M \bra{\ang{T,w_m}^2 \frac{ \beta _m ^4
%         \sigma _m ^2 }{\pa{\sigma _m ^2 + \alpha \beta _m ^2} ^3 } }}
%   { \sum _{m=1} ^M \bra{ \frac{ \beta _m \sigma _m}{\sigma _m ^2 +
%         \alpha \beta _m ^2} \ang{T,w_m} } ^2} }
% }
% {
%     \pa{\pa{
%  { - \frac{\sum _{m=1} ^M \ang{w_m, T}^2 \bra{ \frac{\alpha \sigma _m
%         ^2 \beta _m ^4}{\pa{\sigma _m ^2 + \alpha \beta_m ^2}^3} }} {
%     \sum _{m=1} ^M \bra{ \ang{w_m, T}  \frac{\alpha \beta _m ^2}{ \sigma
%           _m ^2 + \alpha \beta _m ^2 }   } ^2  } }
% } ^2 + \pa{ 
%  { - \frac{ \sum _{m=1} ^M \bra{\ang{T,w_m}^2 \frac{ \beta _m ^4
%         \sigma _m ^2 }{\pa{\sigma _m ^2 + \alpha \beta _m ^2} ^3 } }}
%   { \sum _{m=1} ^M \bra{ \frac{ \beta _m \sigma _m}{\sigma _m ^2 +
%         \alpha \beta _m ^2} \ang{T,w_m} } ^2} }
%  } ^2 } ^ {\sfrac{3}{2}}}
% \end{align*}


\begin{align*}
  \kappa (\alpha) = & \frac{ \rho ' \eta ''  - \rho '' \eta '}{
    \pa{\pa{\rho ' } ^2 + \pa{ \eta ' } ^2 } ^ {\sfrac{3}{2}}} \\
  = &  \frac{ \frac{f'}{2f} \frac{h''h - \pa{h'} ^2}{2h^2}  - \frac{f''f -
      \pa{f'} ^2}{2f^2} \frac{h'}{2h}}  
  { \pa{\pa{\frac{f'}{2f} } ^2 + \pa{ \frac{h'}{2h} } ^2 } ^
    {\sfrac{3}{2}}} = \\
  = & 2fh \frac{f'h\pa{h'' - \pa{h'}^2} - fh' \pa{f'' -
      \pa{f'}^2}}{\bra{\pa{f'}^2 + \pa{h'} ^2 }^{\sfrac{3}{2}}}
\end{align*}




\end{document}